compiler/src/compilerExamples/memequal.v
@@ -6,257 +6,139 @@ Require Import bedrock2.NotationsCustomEntry coqutil.Macros.WithBaseName.
 Require Import compiler.ExprImp.
 Require Import compiler.NameGen.
 Require Import compiler.Pipeline.
+Require Import riscv.Spec.Decode.
+Require Import riscv.Utility.Words32Naive.
+Require Import riscv.Utility.DefaultMemImpl32.
+Require Import riscv.Utility.Monads.
+Require Import compiler.util.Common.
+Require Import coqutil.Decidable.
+Require        riscv.Utility.InstructionNotations.
+Require Import riscv.Platform.MinimalLogging.
+Require Import bedrock2.MetricLogging.
+Require Import riscv.Platform.MetricMinimal.
+Require Import riscv.Utility.Utility.
+Require Import riscv.Utility.Encode.
+Require Import coqutil.Map.SortedList.
+Require Import coqutil.Tactics.fwd.
+Require Import compiler.MemoryLayout.
+Require Import compiler.StringNameGen.
+Require Import riscv.Utility.InstructionCoercions.
+Require Import riscv.Platform.MetricRiscvMachine.
 Require Import riscv.Spec.LeakageOfInstr.
 Require Import riscv.Spec.Decode.
-Require Import riscv.Utility.Words32Naive.
-Require Import riscv.Utility.DefaultMemImpl32.
-Require Import riscv.Utility.Monads.
-Require Import compiler.util.Common.
-Require Import coqutil.Decidable.
-Require        riscv.Utility.InstructionNotations.
-Require Import riscv.Platform.MinimalLogging.
-Require Import bedrock2.MetricLogging.
-Require Import riscv.Platform.MetricMinimal.
-Require Import riscv.Utility.Utility.
-Require Import riscv.Utility.Encode.
-Require Import coqutil.Map.SortedList.
-Require Import compiler.MemoryLayout.
-Require Import compiler.StringNameGen.
-Require Import riscv.Utility.InstructionCoercions.
-Require Import riscv.Platform.MetricRiscvMachine.
-Require bedrock2.Hexdump.
-(*Require Import bedrock2Examples.swap.
-Require Import bedrock2Examples.stackalloc.*)
-Require Import compilerExamples.SpillingTests.
-
-Require Import Coq.Lists.List.
-Import ListNotations.
-Require bedrock2Examples.Demos.
-Require Import coqutil.Decidable.
-Require Import bedrock2.NotationsCustomEntry coqutil.Macros.WithBaseName.
-Require Import compiler.ExprImp.
-Require Import compiler.NameGen.
-Require Import compiler.Pipeline.
-Require Import riscv.Spec.Decode.
-Require Import riscv.Utility.Words32Naive.
-Require Import riscv.Utility.DefaultMemImpl32.
-Require Import riscv.Utility.Monads.
-Require Import compiler.util.Common.
-Require Import coqutil.Decidable.
-Require        riscv.Utility.InstructionNotations.
-Require Import riscv.Platform.MinimalLogging.
-Require Import bedrock2.MetricLogging.
-Require Import riscv.Platform.MetricMinimal.
-Require Import riscv.Utility.Utility.
-Require Import riscv.Utility.Encode.
-Require Import coqutil.Map.SortedList.
-Require Import compiler.MemoryLayout.
-Require Import compiler.StringNameGen.
-Require Import riscv.Utility.InstructionCoercions.
-Require Import riscv.Platform.MetricRiscvMachine.
-Require bedrock2.Hexdump.
-(*Require Import bedrock2Examples.swap.
-Require Import bedrock2Examples.stackalloc.*)
-Require Import compilerExamples.SpillingTests.
 Require compiler.NaiveRiscvWordProperties.
-
+Require Import bedrock2Examples.memequal.
+Require Import compiler.MMIO.
+Require Import bedrock2.FE310CSemantics.
+Require Import coqutil.Map.SortedListZ.
 Require Import compiler.util.Common.
 
-
-Open Scope Z_scope.
-Open Scope string_scope.
-Open Scope ilist_scope.
-
-Definition var: Set := Z.
-Definition Reg: Set := Z.
-
-
-Local Existing Instance DefaultRiscvState.
-
-Local Instance funpos_env: map.map string Z := SortedListString.map _.
+Open Scope Z_scope. Open Scope string_scope. Open Scope ilist_scope.
 
 Notation RiscvMachine := MetricRiscvMachine.
 
 Local Existing Instance coqutil.Map.SortedListString.map.
 Local Existing Instance coqutil.Map.SortedListString.ok.
+Local Instance mem32 : map.map Words32Naive.word Init.Byte.byte := SortedListWord.map Words32Naive.word byte.
+Local Instance mem32_ok : map.ok mem32 := SortedListWord.ok _ _.
+Local Instance localsL32 : map.map Z Words32Naive.word := SortedListZ.map Words32Naive.word.
+Local Instance localsL32_ok : map.ok localsL32 := SortedListZ.ok _.
+Local Instance localsH32: map.map string Words32Naive.word := SortedListString.map Words32Naive.word.
+Local Instance localsH32_ok : map.ok localsH32 := SortedListString.ok _.
+Local Instance RV32I_bitwidth: FlatToRiscvCommon.bitwidth_iset 32 RV32I := eq_refl.
 
-Print compiler_correct_wp.
-Print ExtSpec.
-Section WithParameters.
-  (*Context {mem : map.map Words32Naive.word byte}.
-  Context {mem_ok : map.ok mem}.*)
-
-  Search (map.map _ _).
-  
-  Print funpos_env.
-  Definition mem32 := SortedListWord.map Words32Naive.word byte.
-  Existing Instance mem32.
-  Search SortedListWord.map.
-  Definition mem32_ok : map.ok mem32 := SortedListWord.ok _ _.
-  Existing Instance mem32_ok.
-  Require Import coqutil.Map.SortedListZ.
-
-  Definition localsL32 := SortedListZ.map Words32Naive.word.
-  Existing Instance localsL32.
-  Definition localsL32_ok : map.ok localsL32 := SortedListZ.ok _.
-  Existing Instance localsL32_ok.
-
-  Definition localsH32 := SortedListString.map Words32Naive.word.
-  Existing Instance localsH32.
-  Definition localsH32_ok : map.ok localsH32 := SortedListString.ok _.
-  Existing Instance localsH32_ok.
-  
-  (*Context {localsL : map.map Z Words32Naive.word}.
-  Context {localsL_ok : map.ok localsL}.
-  Context {localsH : map.map string Words32Naive.word}.
-  Context {localsH_ok : map.ok localsH}.
-  Context {envL : map.map string (list Z * list Z * FlatImp.stmt Z)}.
-  Context {envH : map.map string (list string * list string * cmd)}.
-  Context {envH_ok : map.ok envH}.*)
-  (*Context {M : Type -> Type} {MM : Monad M}.*)
-  (*Context {RVM: RiscvProgramWithLeakage}.
-Context {PRParams: PrimitivesParams M MetricRiscvMachine}.
-Context {PR: MetricPrimitives PRParams}.*)
-
-  Require Import compiler.MMIO.
-  Import bedrock2.FE310CSemantics.
-
-  Print compile_ext_call.
-  Local Instance RV32I_bitwidth: FlatToRiscvCommon.bitwidth_iset 32 RV32I.
-  Proof. reflexivity. Qed.
-
-  Check (@FlatToRiscvCommon.compiles_FlatToRiscv_correctly RV32I _ _ _ _ _ compile_ext_call
-           leak_ext_call _ _ _ _ _ _ _ _ compile_ext_call).
-  Check @compiler_correct_wp.
-  (*Check (@PrimitivesParams _ _ _ _ _ M MetricRiscvMachine).
-Check (@compiler_correct_wp _ _ Words32Naive.word mem _ ext_spec _ _ _ _ ext_spec_ok _ _ _ _ _).*)
-  Check NaiveRiscvWordProperties.naive_word_riscv_ok.
-  Lemma word_ok : RiscvWordProperties.word.riscv_ok Words32Naive.word.
-  Proof.
-    cbv [Words32Naive.word]. replace 32 with (2 ^ BinInt.Z.of_nat 5) by reflexivity.
-    apply NaiveRiscvWordProperties.naive_word_riscv_ok.
-  Qed.
-
-  Lemma word_ok' : word.ok Words32Naive.word.
-  Proof.
-    Search (word.ok _). cbv [Words32Naive.word]. exact Naive.word32_ok. Qed.
-
-  Check compile_ext_call_correct.
-
-  (*Lemma compile_ext_call_works :
-  (forall (resvars : list Z) (extcall : string) (argvars : list Z),
-        @FlatToRiscvCommon.compiles_FlatToRiscv_correctly RV32I 32 Bitwidth32.BW32
-          Words32Naive.word localsL (SortedListString.map Z) (@compile_ext_call SortedListString.map) (@leak_ext_call Words32Naive.word SortedListString.map) mem
-          (SortedListString.map (list Z * list Z * FlatImp.stmt Z)) M MM RVM PRParams ext_spec
-          leak_ext RV32I_bitwidth compile_ext_call (@FlatImp.SInteract Z resvars extcall argvars)).
+Lemma word_ok : RiscvWordProperties.word.riscv_ok Words32Naive.word.
 Proof.
-  intros. Search compile_ext_call. cbv [FlatToRiscvCommon.compiles_FlatToRiscv_correctly]. intros.
-  apply compile_ext_call_correct. exfalso. clear -H.
-  inversion H. subst. cbv [ext_spec] in *. assumption.
-Qed.*)
+  cbv [Words32Naive.word]. replace 32 with (2 ^ BinInt.Z.of_nat 5) by reflexivity.
+  apply NaiveRiscvWordProperties.naive_word_riscv_ok.
+Qed.
 
-  Lemma compile_ext_call_length :
-    (forall (stackoffset : Z) (posmap1 posmap2 : SortedListString.map Z) 
-       (c : FlatImp.stmt Z) (pos1 pos2 : Z),
-        @Datatypes.length Instruction (compile_ext_call posmap1 pos1 stackoffset c) =
-          @Datatypes.length Instruction (compile_ext_call posmap2 pos2 stackoffset c)).
-  Proof.
-    intros. cbv [compile_ext_call]. reflexivity. Qed.
+Lemma word_ok' : word.ok Words32Naive.word.
+Proof. exact Naive.word32_ok. Qed.
 
-  Require Import bedrock2Examples.memequal.
+Definition fs_memequal := &[,memequal].
+Definition instrs_memequal :=
+  match (compile compile_ext_call fs_memequal) with
+  | Success (instrs, _, _) => instrs
+  | _ => nil
+  end.
+Definition finfo_memequal :=
+  match (compile compile_ext_call fs_memequal) with
+  | Success (_, finfo, _) => finfo
+  | _ => nil
+  end.
+Definition req_stack_size_memequal :=
+  match (compile compile_ext_call fs_memequal) with
+  | Success (_, _, req_stack_size) => req_stack_size
+  | _ => 0
+  end.
+Definition fname_memequal := "memequal".
+Definition f_rel_pos_memequal := 0.
+Definition post : list LogItem -> mem32 -> list Words32Naive.word -> Prop := fun _ _ _ => True.
 
-  Definition fs_memequal := &[,memequal].
-  Definition instrs_memequal :=
-    match (compile compile_ext_call fs_memequal) with
-    | Success (instrs, _, _) => instrs
-    | _ => nil
-    end.
-  Compute instrs_memequal.
-  Definition finfo_memequal :=
-    match (compile compile_ext_call fs_memequal) with
-    | Success (_, finfo, _) => finfo
-    | _ => nil
-    end.
-  Definition req_stack_size_memequal :=
-    match (compile compile_ext_call fs_memequal) with
-    | Success (_, _, req_stack_size) => req_stack_size
-    | _ => 0
-    end.
-  Definition fname_memequal := "memequal".
-  Definition f_rel_pos_memequal := 0.
-  Definition post : list LogItem -> mem32 -> list Words32Naive.word -> Prop := fun _ _ _ => True.
-  
-  Print spec_of_memequal.
-  Check compiler_correct_wp.
+Lemma memequal_ct :
+  forall x y n p_funcs stack_hi ret_addr,
+  exists finalTrace : list LeakageEvent,
+  forall Rx Ry xs ys m stack_lo
+    Rdata Rexec (initial : RiscvMachine),
+    Separation.sep (Array.array Separation.ptsto (word.of_Z 1) x xs) Rx m /\
+      Separation.sep (Array.array Separation.ptsto (word.of_Z 1) y ys) Ry m /\
+      Z.of_nat (Datatypes.length xs) = word.unsigned n /\
+      Z.of_nat (Datatypes.length ys) = word.unsigned n /\
+      req_stack_size_memequal <= word.unsigned (word.sub stack_hi stack_lo) / SeparationLogic.bytes_per_word ->
+    word.unsigned (word.sub stack_hi stack_lo) mod SeparationLogic.bytes_per_word = 0 ->
+    getPc initial = word.add p_funcs (word.of_Z f_rel_pos_memequal) ->
+    initial.(getTrace) = Some [] ->
+    map.get (getRegs initial) RegisterNames.ra = Some ret_addr ->
+    word.unsigned ret_addr mod 4 = 0 ->
+    LowerPipeline.arg_regs_contain (getRegs initial) [x; y; n] ->
+    LowerPipeline.machine_ok p_funcs stack_lo stack_hi instrs_memequal m Rdata Rexec initial ->
+    FlatToRiscvCommon.runsTo initial
+      (fun final : RiscvMachine =>
+         (exists mH' (retvals : list Words32Naive.word),
+             LowerPipeline.arg_regs_contain (getRegs final) retvals /\
+               post (getLog final) mH' retvals /\
+               map.only_differ (getRegs initial) reg_class.caller_saved (getRegs final) /\
+               getPc final = ret_addr /\
+               final.(getTrace) = Some finalTrace /\
+               LowerPipeline.machine_ok p_funcs stack_lo stack_hi instrs_memequal mH' 
+                 Rdata Rexec final)).
+Proof.
+  assert (spec := @memequal_ok _ _ Words32Naive.word mem32 (SortedListString.map (@Naive.rep 32)) leakage_ext_spec).
+  intros.
+  edestruct (@compiler_correct_wp _ _ Words32Naive.word mem32 _ leakage_ext_spec _ _ _ leakage_ext_spec_ok _ _ _ _ _ word_ok _ _ RV32I _ compile_ext_call leak_ext_call compile_ext_call_correct ltac:(reflexivity) fs_memequal instrs_memequal finfo_memequal req_stack_size_memequal fname_memequal p_funcs stack_hi ret_addr f_rel_pos_memequal) as [f_ [pick_sp_ H] ].
+  { simpl. reflexivity. }
+  { vm_compute. reflexivity. }
+  specialize (spec pick_sp_ word_ok' _ ltac:(apply SortedListString.ok) leakage_ext_spec_ok).
+  cbv [LeakageProgramLogic.program_logic_goal_for] in spec.
+  specialize (spec (map.of_list fs_memequal) eq_refl).
+  cbv [spec_of_memequal] in spec. destruct spec as [f spec].
+  eexists. intros.
+  cbv [FlatToRiscvCommon.runsTo].
+  eapply runsToNonDet.runsTo_weaken.
+  1: eapply H with (post := (fun k_ t_ m_ r_ mc => k_ = _ /\
+                                                  post t_ m_ r_)).
+  { simpl. repeat constructor. tauto. }
+  2: { eapply map.get_of_list_In_NoDup.
+       { vm_compute. repeat constructor; eauto. }
+       { vm_compute. left. reflexivity. } }
+  all: try eassumption.   
+  2: { fwd. assumption. }
 
-  Print spec_of_memequal.
-  Require Import coqutil.Tactics.fwd.
-
-  Lemma memequal_ct :
-    forall x y n p_funcs stack_hi ret_addr,
-    exists finalTrace : list LeakageEvent,
-    forall Rx Ry xs ys m stack_lo
-      Rdata Rexec (initial : RiscvMachine),
-      Separation.sep (Array.array Separation.ptsto (word.of_Z 1) x xs) Rx m /\
-        Separation.sep (Array.array Separation.ptsto (word.of_Z 1) y ys) Ry m /\
-        Z.of_nat (Datatypes.length xs) = word.unsigned n /\
-        Z.of_nat (Datatypes.length ys) = word.unsigned n /\
-        req_stack_size_memequal <= word.unsigned (word.sub stack_hi stack_lo) / SeparationLogic.bytes_per_word ->
-      word.unsigned (word.sub stack_hi stack_lo) mod SeparationLogic.bytes_per_word = 0 ->
-      getPc initial = word.add p_funcs (word.of_Z f_rel_pos_memequal) ->
-      initial.(getTrace) = Some [] ->
-      map.get (getRegs initial) RegisterNames.ra = Some ret_addr ->
-      word.unsigned ret_addr mod 4 = 0 ->
-      LowerPipeline.arg_regs_contain (getRegs initial) [x; y; n] ->
-      LowerPipeline.machine_ok p_funcs stack_lo stack_hi instrs_memequal m Rdata Rexec initial ->
-      FlatToRiscvCommon.runsTo initial
-        (fun final : RiscvMachine =>
-           (exists mH' (retvals : list Words32Naive.word),
-               LowerPipeline.arg_regs_contain (getRegs final) retvals /\
-                 post (getLog final) mH' retvals /\
-                 map.only_differ (getRegs initial) reg_class.caller_saved (getRegs final) /\
-                 getPc final = ret_addr /\
-                 final.(getTrace) = Some finalTrace /\
-                 LowerPipeline.machine_ok p_funcs stack_lo stack_hi instrs_memequal mH' 
-                   Rdata Rexec final)).
-  Proof.
-    assert (spec := @memequal_ok _ _ Words32Naive.word mem32 (SortedListString.map (@Naive.rep 32)) leakage_ext_spec).
-    intros.
-    edestruct (@compiler_correct_wp _ _ Words32Naive.word mem32 _ leakage_ext_spec _ _ _ leakage_ext_spec_ok _ _ _ _ _ word_ok _ _ RV32I _ compile_ext_call leak_ext_call compile_ext_call_correct compile_ext_call_length fs_memequal instrs_memequal finfo_memequal req_stack_size_memequal fname_memequal p_funcs stack_hi ret_addr f_rel_pos_memequal) as [f_ [pick_sp_ H] ].
-    { simpl. reflexivity. }
-    { vm_compute. reflexivity. } Search SortedListString.map.
-    specialize (spec pick_sp_ word_ok' _ ltac:(apply SortedListString.ok) leakage_ext_spec_ok).
-    cbv [LeakageProgramLogic.program_logic_goal_for] in spec.
-    specialize (spec (map.of_list fs_memequal) eq_refl).
-    cbv [spec_of_memequal] in spec. destruct spec as [f spec].
-    eexists. (*exists (rev (f_ (rev (f a_addr b_addr)))).*) intros.
-    cbv [FlatToRiscvCommon.runsTo].
-    eapply runsToNonDet.runsTo_weaken.
-    1: eapply H with (post := (fun k_ t_ m_ r_ mc => k_ = _ /\
-                                                    post t_ m_ r_)).
-    { exact EmptyMetricLog. }
-    { simpl. repeat constructor. tauto. }
-    2: { eapply map.get_of_list_In_NoDup.
-         { vm_compute. repeat constructor; eauto. }
-         { vm_compute. left. reflexivity. } }
-    all: try eassumption.   
-    2: { fwd. assumption. }
-
-    { subst. cbv [fname_memequal]. move spec at bottom.
-      specialize (spec x y n xs ys Rx Ry [] (initial.(getLog)) m ltac:(intuition eauto)).
-      eapply MetricLeakageSemantics.weaken_call.
-      { eapply MetricLeakageSemantics.to_leakage_call. exact spec. }
-      cbv beta. intros. fwd. split; [|reflexivity]. reflexivity. }
-    { reflexivity. }
-    { reflexivity. }
-    cbv beta. intros. fwd. do 2 eexists. intuition eauto.
-    Unshelve. exact EmptyMetricLog.
-  Qed.
-  Print Assumptions memequal_ct.
+  { subst. cbv [fname_memequal]. move spec at bottom.
+    specialize (spec x y n xs ys Rx Ry [] (initial.(getLog)) m ltac:(intuition eauto)).
+    eapply MetricLeakageSemantics.weaken_call.
+    { eapply MetricLeakageSemantics.to_leakage_call. exact spec. }
+    cbv beta. intros. fwd. split; [|reflexivity]. reflexivity. }
+  { reflexivity. }
+  { reflexivity. }
+  cbv beta. intros. fwd. do 2 eexists. intuition eauto.
+  Unshelve. exact EmptyMetricLog.
+Qed.
+(* Print Assumptions memequal_ct. *)
 (*
   Axioms:
   PropExtensionality.propositional_extensionality : forall P Q : Prop, P <-> Q -> P = Q
   FunctionalExtensionality.functional_extensionality_dep :
   forall (A : Type) (B : A -> Type) (f g : forall x : A, B x), (forall x : A, f x = g x) -> f = g
  *)
-End WithParameters.
