compiler/src/compiler/DeadCodeElimDef.v
@@ -1,3 +1,6 @@
+Require Import Coq.Init.Wf Wellfounded.
+Require Import compiler.FixEq.
+Require Import bedrock2.LeakageSemantics.
 Require Import compiler.FlatImp.
 Require Import Coq.Lists.List. Import ListNotations.
 Require Import bedrock2.Syntax.
@@ -14,8 +17,6 @@ Require Import coqutil.Tactics.fwd.
 (*  below only for of_list_list_diff *)
 Require Import Coq.Logic.PropExtensionality.
 Require Import Coq.Logic.FunctionalExtensionality.
-
-Require Import compiler.CustomFix.
 
 Section WithArguments1.
   Context {width: Z}.
@@ -468,12 +469,13 @@ Section WithArguments1.
           SSkip
     | SStackalloc x n body =>
         SStackalloc x n (dce body u)
-        (* The below optimization probably can be made to work;
-           on past attempt, got stuck at goals about `Memory.anybytes n a map.empty` *)
-        (* if (existsb (eqb x) (live body u)) then
-          SStackalloc x n (dce body u)
-        else
-          (dce body u) *)
+    (* Finite address spaces are subtle, so the below optimization is unsound.  See
+       https://github.com/mit-plv/bedrock2/pull/393#discussion_r1685645179*)
+
+    (* if (existsb (eqb x) (live body u)) then
+       SStackalloc x n (dce body u)
+       else
+       (dce body u) *)
     | SLit x _ =>
         if (existsb (eqb x) u) then
           s
@@ -505,9 +507,6 @@ Section WithArguments1.
     | SSkip => SSkip
     end.
 
-  Require Import compiler.CustomFix.
-  Require Import bedrock2.LeakageSemantics.
-  Require Import Coq.Init.Wf Wellfounded.
   Definition tuple : Type := leakage * stmt var * list var * (leakage (*skip*) -> leakage (*everything*)).
   Definition project_tuple (tup : tuple) :=
     let '(kH, s, u, f) := tup in (length kH, s).
@@ -519,26 +518,6 @@ Section WithArguments1.
     cbv [lt_tuple]. apply wf_inverse_image. apply lt_tuple'_wf.
   Defined.
 
-  (*Because high-level pick_sp is always the result of applying low-level pick_sp to
-    low-level trace, this function doesn't need to return a triple
-    (high-level-trace-to-skip, low-level-trace-so-far, high-level-pick-sp-output),
-    like the FlatToRiscv function does.  It suffices to return the first two elts
-    of the tuple.  Nope never mind, we still need the triple, because we need to exit
-    immediately upon hitting a stackalloc; can't continue adding on low-level trace.
-    The third element of the triple could just be an 'error'/'quit'/'exit' boolean,
-    I suppose.  I guess I'll do that?
-
-    We wouldn't have this problem if this thing were written in CPS...
-    But that comes with its own inconveniences in proof-writing:
-    I recall a lot of fumbling around with existential arguments to the continuation.
-    Also I would have to use the custom fix thing (or unnecessarily use functional
-    extensionality) to prove the fixpoint equation.  And I suppose it makes the thing
-    harder to understand for no good reason.
-
-    I guess the best option is the 'error'/short_circuit boolean.
-
-    Nope, I changed my mind.  CPS is good.
-   *)
   Definition stmt_leakage_body
     (e: env)
     (tup : leakage * stmt var * list var * (leakage -> leakage))
@@ -600,14 +579,14 @@ Section WithArguments1.
                     | leak_unit :: kH' =>
                         fun _ => leak_unit :: dtransform_stmt_trace (kH', body, u,
                                   fun skip => f (leak_unit :: skip)) _
-                    | _ => fun _ => nil (*we don't call the continuation here.  wow, that was so much easier than carrying around the 'error' flag*)
+                    | _ => fun _ => nil
                     end eq_refl
               | SLit x _ => fun _ => f nil
               | SOp x op _ _ =>
                   fun _ =>
                     (*copied from spilling.
-                      I should do a leak_list for ops (or just make every op leak two words)
-                      so I don't have to deal with this nonsense*)
+                      Maybe I should do a leak_list for ops (or just make every op leak two words)
+                      to avoid this awkwardness*)
                     let skip :=
                       match op with
                       | Syntax.bopname.divu
