compiler/src/compiler/memory_mapped_ext_calls_riscv.v
@@ -139,7 +139,6 @@ Section Riscv.
 
   Definition setReg(reg: Z)(v: word)(regs: Registers): Registers :=
     if ((0 <? reg) && (reg <? 32)) then map.put regs reg v else regs.
-  Print riscv_primitive.
 
   Definition interpret_action (a : riscv_primitive) (mach : RiscvMachine) :
     (primitive_result a -> RiscvMachine -> Prop) -> (RiscvMachine -> Prop) -> Prop :=
